started work on progress proof

etc.lean
@@ -2,79 +2,151 @@ import .syntax
 
 -- p → q: prop
 
+@[reducible]
 def prop.implies(p q: prop): prop := prop.or (prop.not p) q
 
--- use • as hole
+@[reducible]
+def propctx.implies(p q: propctx): propctx := propctx.or (propctx.not p) q
 
+-- P & Q
+class has_and (α : Type) := (and : α → α → α) 
+instance : has_and prop := ⟨prop.and⟩
+instance : has_and propctx := ⟨propctx.and⟩
+infix `&`:10 := has_and.and
+
+-- use • as hole
 notation `•` := termctx.hole
 
--- simple coersions
-
-instance : has_coe value exp := ⟨exp.value⟩
-instance : has_coe value term := ⟨term.value⟩
+-- simple coercions
+instance : has_coe var term := ⟨term.var⟩
 instance : has_coe term prop := ⟨prop.term⟩
 instance : has_coe termctx propctx := ⟨propctx.term⟩
 
 -- use (t ≡ t)/(t ≣ t) to construct equality comparison
-
 infix ≡ := term.binop binop.eq
 infix `≣`:50 := termctx.binop binop.eq
 
--- term to termctx coersion
+-- syntax for let expressions
+notation `lett` x `=`:1 `true` `in` e := exp.true x e
+notation `letf` x `=`:1 `false` `in` e := exp.false x e
+notation `letn` x `=`:1 n`in` e := exp.num x n e
+notation `letf` f `[`:1 x `]` `req` R `ens` S `{`:1 e `}`:1 `in` e' := exp.func f x R S e e'
+notation `letop` y `=`:1 op `[`:1 x `]`:1 `in` e := exp.unop y op x e
+notation `letop2` z `=`:1 op `[`:1 x `,` y `]`:1 `in` e := exp.binop z op x y e
+notation `letapp` y `=`:1 f `[`:1 x `]`:1 `in` e := exp.app y f x e
+
+-- σ[x ↦ v]
+notation e `[` x `↦` v `]` := env.cons x v e
+
+-- κ · [σ, let y = f [ x ] in e]
+notation st `·` `[` env `,` `let` y `=`:1 f `[` x `]` `in` e `]` := stack.cons st env y f x e
+
+-- (σ, e) : stack
+instance : has_coe (env × exp) stack := ⟨λe, stack.top e.1 e.2⟩
+
+-- env lookup as function application
+
+@[reducible]
+def env.size: env → ℕ := env.rec (λ_, ℕ) 0 (λ_ _ _ n, n + 1)
+instance : has_sizeof env := ⟨env.size⟩
+
+lemma subenv_smaller (σ: env) (x: var) (v: value): σ.size < (σ[x ↦ v].size) :=
+  have σ.size ≤ σ.size, by refl,
+  lt_add_of_le_of_pos this zero_lt_one
+
+def env.apply: env → var → option value
+| env.empty _ := none
+| (σ[x↦v]) y :=
+  have σ.size < (σ[x ↦ v].size), from subenv_smaller σ x v,
+  if x = y then v else env.apply σ y
+
+instance : has_coe_to_fun env := ⟨λ _, var → option value, env.apply⟩
+
+inductive env.contains: env → var → Prop
+| same {e: env} {x: var} {v: value} : env.contains (e[x↦v]) x 
+| rest {e: env} {x y: var} {v: value} : env.contains e x → env.contains (e[y↦v]) x
+
+instance : has_mem var env := ⟨λx σ, σ.contains x⟩ 
+
+-- spec to prop coercion
+
+def spec.to_prop : spec → prop
+| (spec.term t)       := prop.term t
+| (spec.not S)        := prop.not S.to_prop
+| (spec.and R S)      := R.to_prop & S.to_prop
+| (spec.or R S)       := prop.or R.to_prop S.to_prop
+| (spec.func f x R S) :=
+  (term.unop unop.isFunc f) &
+  (prop.forallc x f (prop.implies R.to_prop (prop.pre f x)
+                   & prop.implies (R.to_prop & prop.post f x) S.to_prop))
+
+instance spec_to_prop : has_coe spec prop := ⟨spec.to_prop⟩
+
+-- term to termctx coercion
 
 def term.to_termctx : term → termctx
-| (term.value v) := termctx.value v
-| (term.var x) := termctx.var x
-| (term.unop op t) := termctx.unop op t.to_termctx
+| term.true             := termctx.true
+| term.false            := termctx.false
+| (term.num n)          := termctx.num n
+| (term.var x)          := termctx.var x
+| (term.unop op t)      := termctx.unop op t.to_termctx
 | (term.binop op t₁ t₂) := termctx.binop op t₁.to_termctx t₂.to_termctx
-| (term.app t₁ t₂) := termctx.app t₁.to_termctx t₂.to_termctx
+| (term.app t₁ t₂)      := termctx.app t₁.to_termctx t₂.to_termctx
 
 instance term_to_termctx : has_coe term termctx := ⟨term.to_termctx⟩
 
--- term to termctx coersion
+-- term to termctx coercion
 
 def prop.to_propctx : prop → propctx
-| (prop.term t) := propctx.term t
-| (prop.not p) := propctx.not p.to_propctx
-| (prop.and p₁ p₂) := propctx.and p₁.to_propctx p₂.to_propctx
-| (prop.or p₁ p₂) := propctx.or p₁.to_propctx p₂.to_propctx
-| (prop.pre t₁ t₂) := propctx.pre t₁ t₂
-| (prop.pre₁ op t) := propctx.pre₁ op t
+| (prop.term t)        := propctx.term t
+| (prop.not p)         := propctx.not p.to_propctx
+| (prop.and p₁ p₂)     := p₁.to_propctx & p₂.to_propctx
+| (prop.or p₁ p₂)      := propctx.or p₁.to_propctx p₂.to_propctx
+| (prop.pre t₁ t₂)     := propctx.pre t₁ t₂
+| (prop.pre₁ op t)     := propctx.pre₁ op t
 | (prop.pre₂ op t₁ t₂) := propctx.pre₂ op t₁ t₂
-| (prop.post t₁ t₂) := propctx.post t₁ t₂
-| (prop.call t₁ t₂) := propctx.call t₁ t₂
+| (prop.post t₁ t₂)    := propctx.post t₁ t₂
+| (prop.call t₁ t₂)    := propctx.call t₁ t₂
 | (prop.forallc x t p) := propctx.forallc x t p.to_propctx
-| (prop.univ x p) := propctx.univ x p.to_propctx
-| (prop.exis x p) := propctx.exis x p.to_propctx
+| (prop.exist x p)     := propctx.exist x p.to_propctx
 
 instance prop_to_propctx : has_coe prop propctx := ⟨prop.to_propctx⟩
 
 -- termctx substituttion as function application
 
-def termctx.apply: termctx → var → term
-| •                        x := term.var x
-| (termctx.value v)        _ := v
+def termctx.apply: termctx → term → term
+| •                        t := t
+| termctx.true             _ := term.true
+| termctx.false            _ := term.false
+| (termctx.num n)          _ := term.num n
 | (termctx.var x)          _ := term.var x
-| (termctx.unop op t)      x := term.unop op (t.apply x)
-| (termctx.binop op t₁ t₂) x := term.binop op (t₁.apply x) (t₂.apply x)
-| (termctx.app t₁ t₂)      x := term.app (t₁.apply x) (t₂.apply x)
+| (termctx.unop op t₁)     t := term.unop op (t₁.apply t)
+| (termctx.binop op t₁ t₂) t := term.binop op (t₁.apply t) (t₂.apply t)
+| (termctx.app t₁ t₂)      t := term.app (t₁.apply t) (t₂.apply t)
 
-instance : has_coe_to_fun termctx := ⟨λ _, var → term, termctx.apply⟩
+instance : has_coe_to_fun termctx := ⟨λ _, term → term, termctx.apply⟩
 
 -- propctx substituttion as function application
 
-def propctx.apply: propctx → var → prop
-| (propctx.term t) x := t x
-| (propctx.not p) x := prop.not (p.apply x)
-| (propctx.and p₁ p₂) x := prop.and (p₁.apply x) (p₂.apply x)
-| (propctx.or p₁ p₂) x := prop.or (p₁.apply x) (p₂.apply x)
-| (propctx.pre t₁ t₂) x := prop.or (t₁ x) (t₂ x)
-| (propctx.pre₁ op t) x := prop.pre₁ op (t x)
-| (propctx.pre₂ op t₁ t₂) x := prop.pre₂ op (t₁ x) (t₂ x)
-| (propctx.post t₁ t₂) x := prop.post (t₁ x) (t₂ x)
-| (propctx.call t₁ t₂) x := prop.call (t₁ x) (t₂ x)
-| (propctx.forallc x t p) y := prop.forallc x (t y) (p.apply y)
-| (propctx.univ x p) y := prop.univ x (p.apply y)
-| (propctx.exis x p) y := prop.exis x (p.apply y)
+def propctx.apply: propctx → term → prop
+| (propctx.term t₁) t        := t₁ t
+| (propctx.not p) t          := prop.not (p.apply t)
+| (propctx.and p₁ p₂) t      := (p₁.apply t) & (p₂.apply t)
+| (propctx.or p₁ p₂) t       := prop.or (p₁.apply t) (p₂.apply t)
+| (propctx.pre t₁ t₂) t      := prop.or (t₁ t) (t₂ t)
+| (propctx.pre₁ op t₁) t     := prop.pre₁ op (t₁ t)
+| (propctx.pre₂ op t₁ t₂) t  := prop.pre₂ op (t₁ t) (t₂ t)
+| (propctx.post t₁ t₂) t     := prop.post (t₁ t) (t₂ t)
+| (propctx.call t₁ t₂) t     := prop.call (t₁ t) (t₂ t)
+| (propctx.forallc x t₁ p) t := prop.forallc x (t₁ t) (p.apply t)
+| (propctx.exist x p) t      := prop.exist x (p.apply t)
 
-instance : has_coe_to_fun propctx := ⟨λ _, var → prop, propctx.apply⟩
+instance : has_coe_to_fun propctx := ⟨λ _, term → prop, propctx.apply⟩
+
+-- call history to prop coercion
+
+def calls_to_prop: list call → prop
+| list.nil           := term.true
+| (⟨f, x, y⟩ :: rest) := prop.call f x & prop.post f x & term.app f x ≡ y & calls_to_prop rest
+
+instance call_to_prop: has_coe (list call) prop := ⟨calls_to_prop⟩
