syntax.lean
@@ -17,53 +17,69 @@ inductive binop
 | eq    : binop
 | lt    : binop
 
-mutual inductive value, term, spec, exp
-
-with value: Type
-| num   : ℤ → value
-| true  : value
-| false : value
-| func  : var → var → spec → spec → exp → value
-
-with term: Type
-| value : value → term
+inductive term
+| true  : term
+| false : term
+| num   : ℤ → term
 | var   : var → term
 | unop  : unop → term → term
 | binop : binop → term → term → term
 | app   : term → term → term
 
-with spec: Type
+inductive spec
 | term : term → spec
 | not  : spec → spec
 | and  : spec → spec → spec
 | or   : spec → spec → spec
 | func : term → var → spec → spec → spec
 
+mutual inductive value, env, exp
+
+with value: Type
+| true  : value
+| false : value
+| num   : ℤ → value
+| func  : var → var → spec → spec → exp → env → value
+
+with env: Type
+| empty : env
+| cons  : var → value → env → env -- [x: v, env]
+
 with exp: Type
-| value : value → exp
-| var   : var → exp
-| unop  : unop → exp → exp
-| binop : binop → exp → exp → exp
-| app   : exp → exp → exp
-| ite   : exp → exp → exp → exp
+| true   : var → exp → exp                           -- let x = true in e
+| false  : var → exp → exp                           -- let x = false in e
+| num    : var → ℤ → exp → exp                       -- let x = n in e
+| func   : var → var → spec → spec → exp → exp → exp -- let f(x) R S = e in e
+| unop   : var → unop → var → exp → exp              -- let y = op x in e
+| binop  : var → binop → var → var → exp → exp       -- let z = x op y in e
+| app    : var → var → var → exp → exp               -- let z = x(y) in e
+| ite    : var → exp → exp → exp                     -- if x then e else e
+| return : var → exp                                 -- return x
+
+inductive stack
+| top  : env → exp → stack -- (σ, e)
+| cons : stack → env → var → var → var → exp → stack -- κ · (σ, let y = f(x) in e)
+
+structure call := (f: var) (x: var) (y: var) -- f(x)=y
 
 inductive prop
-| term : term → prop
-| not  : prop → prop
-| and  : prop → prop → prop
-| or   : prop → prop → prop
-| pre  : term → term → prop
-| pre₁ : unop → term → prop
-| pre₂ : binop → term → term → prop
-| post : term → term → prop
-| call : term → term → prop
+| term    : term → prop
+| not     : prop → prop
+| and     : prop → prop → prop
+| or      : prop → prop → prop
+| pre     : term → term → prop
+| pre₁    : unop → term → prop
+| pre₂    : binop → term → term → prop
+| post    : term → term → prop
+| call    : term → term → prop
 | forallc : var → term → prop → prop
-| univ    : var → prop → prop
-| exis : var → prop → prop
+| exist   : var → prop → prop
 
 inductive termctx
 | hole  : termctx
-| value : value → termctx
+| true  : termctx
+| false : termctx
+| num   : ℤ → termctx
 | var   : var → termctx
 | unop  : unop → termctx → termctx
 | binop : binop → termctx → termctx → termctx
@@ -80,5 +96,4 @@ inductive propctx
 | post    : termctx → termctx → propctx
 | call    : termctx → termctx → propctx
 | forallc : var → termctx → propctx → propctx
-| univ    : var → propctx → propctx
-| exis    : var → propctx → propctx
+| exist   : var → propctx → propctx
