vcgen.lean
@@ -2,29 +2,109 @@ import .syntax .etc .props
 
 reserve infix `⊢`:10
 
-inductive vcgen : prop → exp → propctx → Prop
-notation p `⊢` e `:` q : 10 := vcgen p e q
+inductive exp.vcgen : prop → exp → propctx → Prop
+notation P `⊢` e `:` Q : 10 := exp.vcgen P e Q
 
-| num {n: ℤ} {P: prop} :
-    (P ⊢ value.num n : • ≣ value.num n)
+| tru {P: prop} {x: var} {e: exp} {Q: propctx}:
+    x ∉ FV P →
+    (P & x ≡ term.true ⊢ e : Q) →
+    (P ⊢ lett x = true in e : propctx.exist x (x ≡ term.true & Q))
 
-| true {P: prop} :
-    (P ⊢ value.true : • ≣ value.true)
+| fals {P: prop} {x: var} {e: exp} {Q: propctx}:
+    x ∉ FV P →
+    (P & x ≡ term.false ⊢ e : Q) →
+    (P ⊢ letf x = false in e : propctx.exist x (x ≡ term.false & Q))
 
-| false {P: prop} :
-    (P ⊢ value.false : • ≣ value.false)
+| num {P: prop} {x: var} {n: ℕ} {e: exp} {Q: propctx}:
+    x ∉ FV P →
+    (P & x ≡ term.num n ⊢ e : Q) →
+    (P ⊢ letn x = n in e : propctx.exist x (x ≡ term.num n & Q))
 
-| var {P: prop} {x: var} :
-    (P ⊢ exp.var x : term.var r ≡ term.var x)
+| func {P: prop} {f x: var} {R S: spec} {e₁ e₂: exp} {Q₁ Q₂: propctx}:
+    f ∉ FV P →
+    x ∉ FV P →
+    (P & spec.func f x R S & R ⊢ e₂ : Q₂) →
+    ⟪ prop.implies (P & (spec.func f x R S) & R)
+                   (Q₂ (term.app f x)) ⟫ →
+    (P ⊢ letf f[x] req R ens S {e₁} in e₂ :
+         propctx.exist f (spec.func f x R S & Q₁))
 
-| unop {P Q: prop} {op: unop} {e: exp} {x r: var} :
-    (P ⊢ x, e : Q) →
-    ⟪ prop.implies (prop.and P Q) (prop.pre₁ op (term.var x)) ⟫ →
-    (P ⊢ r, exp.unop op e : prop.exis x (prop.and Q (term.var r ≡ term.unop op (term.var x))))
+| unop {P: prop} {op: unop} {e: exp} {x y: var} {Q: propctx}:
+    x ∈ FV P →
+    y ∉ FV P →
+    (P & y ≡ term.unop op x ⊢ e : Q) →
+    ⟪ prop.implies P (prop.pre₁ op x) ⟫ →
+    (P ⊢ letop y = op [x] in e : propctx.exist y (y ≡ term.unop op x & Q))
 
-| unop {P: prop} {Q: propctx} {op: unop} {e: exp} {x: var} :
-    (P ⊢ e : Q) →
-    ⟪ prop.univ x (prop.implies (prop.and P (Q x)) (prop.pre₁ op (term.var x))) ⟫ →
-    (P ⊢ exp.unop op e : propctx.exis x (propctx.and (Q x) (• ≣ term.unop op (term.var x))))
+| binop {P: prop} {op: binop} {e: exp} {x y z: var} {Q: propctx}:
+    x ∈ FV P →
+    y ∈ FV P →
+    z ∉ FV P →
+    (P & z ≡ term.binop op x y ⊢ e : Q) →
+    ⟪ prop.implies P (prop.pre₂ op x y) ⟫ →
+    (P ⊢ letop2 y = op [x, y] in e : propctx.exist y (z ≡ term.binop op x y & Q))
 
-notation p `⊢` r `,` e `:` q : 10 := vcgen p r e q
+| app {P: prop} {e: exp} {y f x: var} {Q: propctx}:
+    f ∈ FV P →
+    x ∈ FV P →
+    y ∉ FV P →
+    (P & prop.call f x & y ≡ term.app f x & prop.post f x ⊢ e : Q) →
+    ⟪ prop.implies (P & prop.call f x) (term.unop unop.isFunc f & prop.pre f x) ⟫ →
+    (P ⊢ letapp y = f [x] in e : propctx.exist y (prop.call f x & y ≡ term.app f x & prop.post f x & Q))
+
+| ite {P: prop} {e₁ e₂: exp} {x: var} {Q₁ Q₂: propctx}:
+    x ∈ FV P →
+    (P & x ⊢ e₁ : Q₁) →
+    (P & term.unop unop.not x ⊢ e₂ : Q₂) →
+    ⟪ prop.implies P (term.unop unop.isBool x) ⟫ →
+    (P ⊢ exp.ite x e₁ e₂ : (propctx.implies x Q₁ & propctx.implies (term.unop unop.not x) Q₂))
+
+| return {P: prop} {op: unop} {e: exp} {x: var}:
+    x ∈ FV P →
+    (P ⊢ exp.return x : x ≣ •)
+
+notation P `⊢` e `:` Q : 10 := exp.vcgen P e Q
+
+inductive env.vcgen : env → prop → Prop
+notation `⊢` σ `:` Q : 10 := env.vcgen σ Q
+
+| empty:
+    ⊢ env.empty : term.true
+
+| tru {σ: env} {x: var} {Q: prop}:
+    (⊢ σ : Q) →
+    (⊢ (σ[x ↦ value.true]) : (Q & x ≡ term.true))
+
+| fls {σ: env} {x: var} {Q: prop}:
+    (⊢ σ : Q) →
+    (⊢ (σ[x ↦ value.false]) : (Q & x ≡ term.false))
+
+| num {σ: env} {x: var} {n: ℤ} {Q: prop}:
+    (⊢ σ : Q) →
+    (⊢ (σ[x ↦ value.num n]) : (Q & x ≡ term.num n))
+
+| func {σ₁ σ₂: env} {f x: var} {R S: spec} {e: exp} {Q₁ Q₂: prop} {Q₃: propctx}:
+    (⊢ σ₁ : Q₁) →
+    (⊢ σ₂ : Q₂) →
+    (Q₂ & spec.func f x R S & R ⊢ e : Q₃) →
+    ⟪ prop.implies (Q₂ & (spec.func f x R S) & R)
+                   (Q₃ (term.app f x)) ⟫ →
+    (⊢ (σ₁[x ↦ value.func f x R S e σ₂]) : (Q₁ & spec.func f x R S))
+
+notation `⊢` σ `:` Q : 10 := env.vcgen σ Q
+
+inductive stack.vcgen : prop → stack → Prop
+notation P `⊩` s : 10 := stack.vcgen P s
+
+| top {P₁ P₂: prop} {σ: env} {e: exp} {Q: propctx}:
+    (⊢ σ : P₂) →
+    (P₁ & P₂ ⊢ e : Q) →
+    (P₁ ⊩ (σ, e))
+
+| cons {P₁ P₂: prop} {s: stack} {σ: env} {f x y: var} {e: exp} {Q: propctx}:
+    (P₁ ⊩ s) →
+    (⊢ σ : P₂) →
+    (P₁ & P₂ ⊢ letapp y = f[x] in e : Q) →
+    (P₁ ⊩ (s · [σ, let y = f[x] in e]))
+
+notation P `⊩` s : 10 := stack.vcgen P s
