progress.lean
@@ -1,0 +1,50 @@
+import .syntax .etc .evaluation .props .vcgen
+
+def is_return(s: stack): Prop := ∃(σ: env) (x: var), s = (σ, exp.return x)
+
+theorem progress(P: prop) (s: stack): ⟪P⟫ ∧ (P ⊩ s) → is_return s ∨ ∃c s', s ⟶ c, s' :=
+  assume ⟨P_valid, s_verified⟩,
+  stack.vcgen.rec_on s_verified
+  ( -- top
+    assume P₁ P₂: prop,
+    assume σ: env,
+    assume e: exp,
+    assume Q: propctx,
+    assume env_verified: (⊢ σ : P₂),
+    assume e_verified: (P₁ & P₂ ⊢ e : Q),
+    let s := (σ, e) in
+    show is_return s ∨ ∃c s', s ⟶ c, s', from sorry
+  )
+  ( -- cons
+    assume P₁ P₂: prop,
+    assume s': stack,
+    assume σ: env,
+    assume f x y: var,
+    assume e: exp,
+    assume Q: propctx,
+    assume s'_verified: P₁ ⊩ s',
+    assume env_verified: ⊢ σ : P₂,
+    assume cont_verified: P₁ & P₂ ⊢ letapp y = f[x] in e : Q,
+    assume ih: is_return s' ∨ ∃c s'', s' ⟶ c, s'',
+    let s := (s' · [σ, let y = f[x] in e]) in
+    have s_cons: s = (s' · [σ, let y = f[x] in e]), from rfl,
+    ih.elim
+    (
+      assume s'_is_return: is_return s',
+      let ⟨σ₂, z, s'_return⟩ := s'_is_return in
+      have s = ((σ₂, exp.return z) · [σ, let y = f[x] in e]), from s'_return ▸ s_cons,
+      have s ⟶ some ⟨f, x, y⟩, (σ[y↦v], e)), from step.return sorry,
+      have s ⟶ c, (s'' · [σ, let y = f[x] in e]), from step.ctx s'_steps,
+      have ∃s', s ⟶ c, s', from exists.intro (s'' · [σ, let y = f[x] in e]) this,
+      have ∃c s', s ⟶ c, s', from exists.intro c this,
+      show is_return s ∨ ∃c s', s ⟶ c, s', from sorry
+    )
+    (
+      assume s'_can_step: ∃c s'', s' ⟶ c, s'',
+      let ⟨c, s'', s'_steps⟩ := s'_can_step in
+      have s ⟶ c, (s'' · [σ, let y = f[x] in e]), from step.ctx s'_steps,
+      have ∃s', s ⟶ c, s', from exists.intro (s'' · [σ, let y = f[x] in e]) this,
+      have ∃c s', s ⟶ c, s', from exists.intro c this,
+      show is_return s ∨ ∃c s', s ⟶ c, s', from or.inr this
+    )
+  )
