props.lean
@@ -1,5 +1,43 @@
 import .syntax .etc
 
+-- free variables
+
+inductive free_in_term (x: var) : term → Prop
+| freevar                          : free_in_term x
+| unop {t: term} {op: unop}        : free_in_term t → free_in_term (term.unop op t)
+| binop₁ {t₁ t₂: term} {op: binop} : free_in_term t₁ → free_in_term (term.binop op t₁ t₂)
+| binop₂ {t₁ t₂: term} {op: binop} : free_in_term t₂ → free_in_term (term.binop op t₁ t₂)
+| app₁ {t₁ t₂: term}               : free_in_term t₁ → free_in_term (term.app t₁ t₂)
+| app₂ {t₁ t₂: term}               : free_in_term t₂ → free_in_term (term.app t₁ t₂)
+
+inductive free_in_prop (x: var) : prop → Prop
+| term {t: term}                        : free_in_term x t → free_in_prop t
+| not {p: prop}                         : free_in_prop p → free_in_prop (prop.not p)
+| and₁ {p₁ p₂: prop}                    : free_in_prop p₁ → free_in_prop (prop.and p₁ p₂)
+| and₂ {p₁ p₂: prop}                    : free_in_prop p₂ → free_in_prop (prop.and p₁ p₂)
+| or₁ {p₁ p₂: prop}                     : free_in_prop p₁ → free_in_prop (prop.or p₁ p₂)
+| or₂ {p₁ p₂: prop}                     : free_in_prop p₂ → free_in_prop (prop.or p₁ p₂)
+| pre₁ {t₁ t₂: term}                    : free_in_term x t₁ → free_in_prop (prop.pre t₁ t₂)
+| pre₂ {t₁ t₂: term}                    : free_in_term x t₂ → free_in_prop (prop.pre t₁ t₂)
+| preop {t: term} {op: unop}            : free_in_term x t → free_in_prop (prop.pre₁ op t)
+| preop₁ {t₁ t₂: term} {op: binop}      : free_in_term x t₁ → free_in_prop (prop.pre₂ op t₁ t₂)
+| preop₂ {t₁ t₂: term} {op: binop}      : free_in_term x t₂ → free_in_prop (prop.pre₂ op t₁ t₂)
+| post₁ {t₁ t₂: term}                   : free_in_term x t₁ → free_in_prop (prop.post t₁ t₂)
+| post₂ {t₁ t₂: term}                   : free_in_term x t₂ → free_in_prop (prop.post t₁ t₂)
+| call₁ {t₁ t₂: term}                   : free_in_term x t₁ → free_in_prop (prop.call t₁ t₂)
+| call₂ {t₁ t₂: term}                   : free_in_term x t₂ → free_in_prop (prop.call t₁ t₂)
+| forallc₁ {y: var} {t: term} {p: prop} : (x ≠ y) → free_in_term x t → free_in_prop (prop.forallc y t p)
+| forallc₂ {y: var} {t: term} {p: prop} : (x ≠ y) → free_in_prop p → free_in_prop (prop.forallc y t p)
+| exist {y: var} {p: prop}              : (x ≠ y) → free_in_prop p → free_in_prop (prop.exist y p)
+
+-- notation x ∈ FV p
+
+structure freevars := (p: prop)
+instance : has_mem var freevars := ⟨λx fv, free_in_prop x fv.p⟩ 
+def FV(p: prop): freevars := freevars.mk p
+
+-- validity
+
 inductive valid : prop → Prop
 notation `⟪` p `⟫`: 100 := valid p
 | to_prop {p: prop}: valid p
